books/projects/rp-rewriter/lib/mult3/lemmas.lisp
@@ -55,12 +55,12 @@
 
 (defthm integerp-m2-f2-d2
   (and (integerp (m2 x))
-       (integerp (d2 x))
+       ;(integerp (d2 x))
        (integerp (f2 x))
        (integerp (sum x y))
        (integerp (sum-list x)))
   :hints (("Goal"
-           :in-theory (e/d (m2 d2 f2 sum-list sum) ()))))
+           :in-theory (e/d (m2  f2 sum-list sum) ()))))
 
 (defthm integerp-ifix
   (integerp (ifix x)))
@@ -68,8 +68,8 @@
 (defthm m2-f2-d2-sum-of-ifix
   (and (equal (f2 (ifix x))
               (f2 x))
-       (equal (d2 (ifix x))
-              (d2 x))
+       #|(equal (d2 (ifix x))
+              (d2 x))||#
        (equal (m2 (ifix x))
               (m2 x))
        (equal (sum (ifix x) b)
@@ -77,7 +77,7 @@
        (equal (sum b (ifix x))
               (sum x b)))
   :hints (("Goal"
-           :in-theory (e/d (m2 f2 d2 sum)
+           :in-theory (e/d (m2 f2 #|d2||# sum)
                            (
                             (:REWRITE ACL2::|(equal (if a b c) x)|)
                             (:REWRITE ACL2::|(floor x 2)| . 1))))))
@@ -98,9 +98,11 @@
        (mv 'm2 x))
       (('f2 &)
        (mv 'f2 x))
-      (('d2 &)
-       (mv 'd2 x))
+      #|(('d2 &)
+       (mv 'd2 x))||#
       (('-- x)
+       (sum-comm-order-aux x (1+ cnt)))
+      (('times2 x)
        (sum-comm-order-aux x (1+ cnt)))
       (('sum-list x)
        (sum-comm-order-aux x (1+ cnt)))
@@ -155,15 +157,15 @@
        ((or (equal a-type 'merge)
             (equal b-type 'merge))
         (not (equal b-type 'merge)))
-       ((or (and (equal a-type 'd2)
-                 (equal b-type 'd2))
+       ((or #|(and (equal a-type 'd2)
+                 (equal b-type 'd2))||#
             (and (equal a-type 'f2)
                  (equal b-type 'f2)))
         (b* (((mv res &) (lexorder2 a b)))
           res))
-       ((or (equal a-type 'd2)
+       #|((or (equal a-type 'd2)
             (equal b-type 'd2))
-        (not (equal a-type 'd2)))
+        (not (equal a-type 'd2)))||#
        ((or (equal a-type 'f2)
             (equal b-type 'f2))
         (not (equal a-type 'f2)))
@@ -611,15 +613,21 @@
   :hints (("Goal"
            :in-theory (e/d (times2) ()))))
 
-(defthm d2-to-f2
+(defthm times2-of-sum
+  (equal (times2 (sum a b))
+         (sum (times2 a) (times2 b)))
+  :hints (("Goal"
+           :in-theory (e/d (times2) ()))))
+
+#|(defthm d2-to-f2
   (and (EQUAL (d2 (sum (-- (m2 x)) x))
               (f2 x))
        (EQUAL (d2 (sum x (-- (m2 x))))
               (f2 x)))
   :hints (("Goal"
-           :in-theory (e/d (sum m2 d2 f2) ()))))
+           :in-theory (e/d (sum m2 d2 f2) ()))))||#
 
-(defthmd f2-to-d2
+#|(defthmd f2-to-d2
   (EQUAL (f2 x)
          (d2 (sum (-- (m2 x)) x)))
   :hints (("Goal"
@@ -628,7 +636,7 @@
                             SUM-COMM-2
                             (:REWRITE ACL2::|(mod x 2)| . 1)
                             (:REWRITE ACL2::|(equal (if a b c) x)|)
-                            (:REWRITE ACL2::|(floor x 2)| . 1))))))
+                            (:REWRITE ACL2::|(floor x 2)| . 1))))))||#
 
 (defthmd equal-sum-of-negated
   (and (equal (equal (sum x y) (sum (-- a) b))
@@ -696,7 +704,7 @@
 (add-invisible-fns binary-sum sum-list)
 (add-invisible-fns binary-sum times2)
 
-(encapsulate
+#|(encapsulate
   nil
 
   (local
@@ -779,24 +787,24 @@
              :in-theory (e/d (f2-to-d2)
                              (d2-to-f2
                               ;D2-OF-MINUS
-                              ))))))
+                              ))))))||#
 
-(defthm evenpi-for-2-d2-arguments
+#|(defthm evenpi-for-2-d2-arguments
   (evenpi (sum a b (-- (m2 (sum a b)))))
   :hints (("Goal"
-           :in-theory (e/d (evenpi sum m2) ()))))
+           :in-theory (e/d (evenpi sum m2) ()))))||#
 
-(defthm evenpi-for-3-d2-arguments
+#|(defthm evenpi-for-3-d2-arguments
   (evenpi (sum a b c (-- (m2 (sum a b c)))))
   :hints (("Goal"
-           :in-theory (e/d (evenpi sum m2) ()))))
+           :in-theory (e/d (evenpi sum m2) ()))))||#
 
-(defthm evenpi-for-4-d2-arguments
+#|(defthm evenpi-for-4-d2-arguments
   (evenpi (sum a b c d (-- (m2 (sum a b c d)))))
   :hints (("Goal"
-           :in-theory (e/d (evenpi sum m2) ()))))
+           :in-theory (e/d (evenpi sum m2) ()))))||#
 
-(defthm evenpi-sum-clear
+#|(defthm evenpi-sum-clear
   (and (equal (evenpi (sum a a b))
               (evenpi (ifix b)))
        (equal (evenpi (sum a a))
@@ -816,7 +824,7 @@
        (equal (evenpi (sum c d e a a))
               (evenpi (sum c d e))))
   :hints (("Goal"
-           :in-theory (e/d (sum evenpi) ()))))
+           :in-theory (e/d (sum evenpi) ()))))||#
 
 (defthm m2-with-extra
   (implies (equal (m2 x) (m2 y))
@@ -855,3 +863,25 @@
 (in-theory (enable +-is-SUM
                    mod2-is-m2
                    floor2-if-f2))
+
+
+(defthm sum-of-negated-elements
+  (implies (equal (-- a) b)
+           (and (equal (sum a b) 0)
+                (equal (sum b a) 0)
+                (equal (sum b a rest) (ifix rest))
+                (equal (sum a b rest) (ifix rest))))
+  :hints (("Goal"
+           :in-theory (e/d (sum --)
+                           (+-IS-SUM)))))
+
+
+(defthmd f2-of-times2-reverse
+  (implies (syntaxp (or (atom term)
+                        (not (equal (car term) 'f2))))
+           (and (equal (sum term (f2 term2))
+                       (f2 (sum (times2 term) term2)))
+                (equal (sum (f2 term2) term)
+                       (f2 (sum (times2 term) term2)))
+                (equal (sum term (f2 term2) other)
+                       (sum other (f2 (sum (times2 term) term2)))))))
